Implemented OR-Set using FStar.Set

inductive_proof/Observed-remove_set/App_comm.fst
@@ -4,16 +4,16 @@ open FStar.Seq
 open FStar.Ghost
 module L = FStar.List.Tot
 
+module S = FStar.Set
+
 #set-options "--query_stats"
 // the concrete state type
-type concrete_st = list (nat (*unique id*) * nat (*element*))
+type concrete_st = S.set (nat * nat)
 
-// init state
-let init_st = []
+let init_st = S.empty
 
-// equivalence between 2 concrete states
 let eq (a b:concrete_st) =
-  (forall ele. L.mem ele a <==> L.mem ele b)
+  (forall ele. S.mem ele a <==> S.mem ele b)
 
 // few properties of equivalence relation
 let symmetric (a b:concrete_st) 
@@ -38,75 +38,23 @@ let get_ele (o:op_t) : nat =
   |Add e -> e
   |Rem e -> e
 
-val mem_id_s : id:nat 
-             -> l:list (nat * nat)
-             -> Tot (b:bool{(exists n. L.mem (id,n) l) <==> b=true})
-let rec mem_id_s n l =
-  match l with
-  |[] -> false
-  |(id,_)::xs -> (n = id) || mem_id_s n xs
+let mem_ele (ele:nat) (s:concrete_st) : prop =
+  (exists id. S.mem (id, ele) s)
 
-val mem_ele : ele:nat 
-            -> l:list (nat * nat)
-            -> Tot (b:bool{(exists n. L.mem (n,ele) l) <==> b=true})
-let rec mem_ele ele l =
-  match l with
-  |[] -> false
-  |(_,ele1)::xs -> (ele = ele1) || mem_ele ele xs
-
-val filter : f:((nat * nat) -> bool)
-           -> l:concrete_st
-           -> Tot (l1:concrete_st {(forall e. L.mem e l /\ f e <==> L.mem e l1)})
-let rec filter f l = 
-  match l with
-  |[] -> []
-  |hd::tl -> if f hd then hd::(filter f tl) else filter f tl
+assume val remove_if (#a:eqtype) (s:S.set a) (f:a -> bool) : S.set a
+assume val remove_if_mem (#a:eqtype) (s:S.set a) (f:a -> bool) (x:a)
+  : Lemma (ensures S.mem x (remove_if s f) <==> (S.mem x s /\ ~ (f x))) 
+    [SMTPat (S.mem x (remove_if s f))]
 
 // apply an operation to a state
-let do (s:concrete_st) (o:op_t) 
-    : (r:concrete_st{(Add? (snd o) ==> (forall ele. mem_ele ele r <==> (mem_ele ele s \/ ele = get_ele o)) /\
-                                      (forall e. L.mem e r <==> (L.mem e s \/ (e = (fst o, get_ele o)))) /\
-                                      (forall id. mem_id_s id r <==> (mem_id_s id s \/ id = fst o)) /\
-                                      (forall e. L.mem e r /\ snd e <> get_ele o <==> L.mem e s /\ snd e <> get_ele o) /\
-                                      r = (fst o, get_ele o)::s) /\
-                     (Rem? (snd o) ==> (forall ele. mem_ele ele r <==> (mem_ele ele s /\ ele <> get_ele o)) /\
-                                      (forall e. L.mem e r <==> (L.mem e s /\ snd e <> get_ele o)) /\
-                                      (forall id. mem_id_s id r ==> mem_id_s id s) /\
-                                      not (mem_ele (get_ele o) r))}) =
+let do (s:concrete_st) (o:op_t) : concrete_st =
   match o with
-  |(id, Add e) -> (id, e)::s
-  |(id, Rem e) -> filter (fun ele -> snd ele <> e) s
-
-let do_prop (s:concrete_st) (o:op_t)
-  : Lemma (ensures (Add? (snd o) ==> ((forall ele. mem_ele ele (do s o) <==> (mem_ele ele s \/ ele = get_ele o)) /\
-                                     (forall e. L.mem e (do s o) <==> (L.mem e s \/ e = (fst o, get_ele o))) /\
-                                     (forall id. mem_id_s id (do s o) <==> (mem_id_s id s \/ id = fst o)) /\
-                                     L.mem (fst o, get_ele o) (do s o) /\
-                                    (forall e. L.mem e (do s o) /\ snd e <> get_ele o <==> L.mem e s /\ snd e <> get_ele o) /\
-                                    (do s o = (fst o, get_ele o)::s ))) /\
-                   (Rem? (snd o) ==> ((forall e. L.mem e (do s o) <==> (L.mem e s /\ snd e <> get_ele o)) /\
-                                     not (mem_ele (get_ele o) (do s o)) /\
-                                    (forall id. mem_id_s id (do s o) ==> mem_id_s id s)))) = ()
-
+  |(id, Add e) -> S.union (S.singleton (id, e)) s
+  |(id, Rem e) -> remove_if s (fun ele -> snd ele = e)
+  
 let lem_do (a b:concrete_st) (op:op_t)
    : Lemma (requires eq a b)
            (ensures eq (do a op) (do b op)) = ()
-           
-val exists_op : f:(op_t -> bool)
-              -> l:log
-              -> Tot (b:bool{(exists e. mem e l /\ f e) <==> b = true}) (decreases length l)
-let rec exists_op f l =
-  match length l with
-  | 0 -> false
-  | _ -> if f (head l) then true else exists_op f (tail l)
-
-val forall_op : f:(op_t -> bool)
-              -> l:log
-              -> Tot (b:bool{(forall e. mem e l ==> f e) <==> b = true}) (decreases length l)
-let rec forall_op f l =
-  match length l with
-  | 0 -> true
-  | _ -> f (head l) && forall_op f (tail l)
 
 //conflict resolution
 let resolve_conflict (x:op_t) (y:op_t{fst x <> fst y}) : (l:log{(forall e. mem e l <==> (e == x \/ e == y))}) =
@@ -125,52 +73,13 @@ let resolve_conflict_prop (x y:op_t)
                                                         (Rem? (snd x) /\ Add? (snd y)))))
   = ()
 
-// remove ele from l
-let rec remove (l:concrete_st) (ele:(nat * nat)) 
-  : Tot (res:concrete_st{(forall e. L.mem e res <==> L.mem e l /\ e <> ele) /\ not (L.mem ele res)}) =
-  match l with
-  |[] -> []
-  |x::xs -> if x = ele then remove xs ele else x::remove xs ele
-
-// a - l
-let diff_s (a l:concrete_st)
-  : Pure (concrete_st) 
-    (requires true)
-    (ensures (fun d -> (forall e. L.mem e d <==> (L.mem e a /\ not (L.mem e l))) /\
-                       (forall ele. (forall e. L.mem e a /\ snd e = ele <==> L.mem e l /\ snd e = ele) ==>
-                               not (mem_ele ele d)) /\
-                       (forall ele. not (mem_ele ele a) ==> not (mem_ele ele d)) /\
-                       (forall e. L.mem e a /\ not (L.mem e l) <==> L.mem e d)))  (decreases a) =
-  filter (fun e -> not (L.mem e l)) a
-
-#push-options "--z3rlimit 200"
-val concrete_merge1 (l a b:concrete_st)
-           : Pure concrete_st
-             (requires true)
-             (ensures (fun res -> (forall e. L.mem e res <==> (L.mem e l /\ L.mem e a /\ L.mem e b) \/ 
-                                                    (L.mem e (diff_s a l)) \/ (L.mem e (diff_s b l))) /\
-                              (forall id. mem_id_s id res ==> (mem_id_s id l \/ mem_id_s id a \/ mem_id_s id b))))
-                               (decreases %[l;a;b])
-let rec concrete_merge1 l a b =
-  match l,a,b with
-  |[],[],[] -> []
-  |x::xs,_,_ -> if (L.mem x a && L.mem x b) then x::(concrete_merge1 xs (remove a x) (remove b x)) 
-                 else if (L.mem x a) then (concrete_merge1 xs (remove a x) b)
-                   else if (L.mem x b) then (concrete_merge1 xs a (remove b x))
-                     else (concrete_merge1 xs a b)
-  |[],x::xs,_ -> x::(concrete_merge1 [] xs b)
-  |[],[],x::xs -> b
-#pop-options
-
-// concrete merge operation
-let concrete_merge (l a b:concrete_st)
-    : Tot (res:concrete_st {(forall e. L.mem e res <==> (L.mem e l /\ L.mem e a /\ L.mem e b) \/ 
-                                                 (L.mem e (diff_s a l)) \/ (L.mem e (diff_s b l))) /\
-                            (l = a ==> (forall e. L.mem e res <==> L.mem e b)) /\
-                            (l = b ==> (forall e. L.mem e res <==> L.mem e a)) /\
-                            (forall b'. eq b b' ==> eq res (concrete_merge1 l a b')) /\
-                            (forall a'. eq a a' ==> eq res (concrete_merge1 l a' b))}) =
- concrete_merge1 l a b
+(*merge l a b == (intersect l a b) U (a - l) U (b - l)*)
+let concrete_merge (l a b:concrete_st) : concrete_st =
+  let da = remove_if a (fun e -> S.mem e l) in
+  let db = remove_if b (fun e -> S.mem e l) in
+  let i_la = S.intersect l a in
+  let i_lab = S.intersect i_la b in
+  S.union i_lab (S.union da db)
 
 //operations x and y are commutative
 let commutative (x y:op_t) =
@@ -212,16 +121,6 @@ let linearizable_s2_0 (lca s1 s2:st)
                     (forall id id1. mem_id id (ops_of lca) /\ mem_id id1 (diff (ops_of s1) (ops_of lca)) ==> lt id id1) /\
                     (forall id id1. mem_id id (ops_of lca) /\ mem_id id1 (diff (ops_of s2) (ops_of lca)) ==> lt id id1))
           (ensures eq (v_of s1) (concrete_merge (v_of lca) (v_of s1) (v_of s2))) = ()
-
-let trans_op (a b c:concrete_st) (ele:(nat * nat))
-  : Lemma (requires (forall e. L.mem e a <==> (L.mem e b \/ e == ele)) /\
-                    (forall e. (L.mem e b \/ e == ele) <==> L.mem e c))
-          (ensures eq a c) = ()
-
-let trans_op_ele (a b c:concrete_st) (ele:nat)
-  : Lemma (requires (forall e. L.mem e a <==> (L.mem e b /\ snd e <> ele)) /\
-                    (forall e. (L.mem e b /\ snd e <> ele) <==> L.mem e c))
-          (ensures eq a c) = ()
 
 type common_pre_s2_gt0 (lca s1 s2:st) =
   is_prefix (ops_of lca) (ops_of s1) /\
@@ -265,17 +164,8 @@ let lem_lca_eq''_base_pre (lca s1 s2:st) (last1 last2:op_t)
                       let s2' = inverse_st s2 in
                       not (mem_id (fst last1) (ops_of l')) /\
                       not (mem_id (fst last2) (ops_of l')) /\
-                      ops_of s1' = ops_of l' /\ ops_of s2' = ops_of l')) =
-  let l' = inverse_st lca in
-  let pre, lastl = un_snoc (ops_of lca) in
-  lemma_mem_append pre (create 1 lastl);
-  assert (mem lastl (ops_of lca)); 
-  lem_mem_ele_mem_id_single lastl (ops_of lca);
-  assert (mem_id (fst lastl) (ops_of lca)); 
-  assert (not (mem_id (fst last1) (ops_of l')) /\
-          not (mem_id (fst last2) (ops_of l')) ); ()
+                      ops_of s1' = ops_of l' /\ ops_of s2' = ops_of l')) = ()
 
-#push-options "--z3rlimit 50"
 let lem_l2a_l1r_eq''_base_ind (lca s1 s2:st) (last1 last2:op_t)
   : Lemma (requires length (ops_of lca) > 0 /\
                     ops_of s1 = ops_of lca /\ ops_of s2 = ops_of lca /\
@@ -292,14 +182,11 @@ let lem_l2a_l1r_eq''_base_ind (lca s1 s2:st) (last1 last2:op_t)
           (ensures eq (do (concrete_merge (v_of lca) (do (v_of s1) last1) (v_of s2)) last2)
                       (concrete_merge (v_of lca) (do (v_of s1) last1) (do (v_of s2) last2))) =
   let pre, lastl = un_snoc (ops_of lca) in
-  lemma_mem_append pre (create 1 lastl); 
-  assert (mem lastl (ops_of lca)); 
   lem_mem_ele_mem_id_single lastl (ops_of lca);
   assert (mem_id (fst lastl) (ops_of lca)); 
   assert (fst lastl <> fst last1);
   assert (fst lastl <> fst last2);
   ()
-#pop-options
 
 let rec lem_l2a_l1r_eq''_base (lca s1 s2:st) (last1 last2:op_t)
   : Lemma (requires ops_of s1 = ops_of lca /\ ops_of s2 = ops_of lca /\
@@ -328,7 +215,7 @@ let lem_l2a_l1r_eq''_s10_s2_gt0 (lca s1 s2:st) (last1 last2:op_t)
                         (concrete_merge (v_of lca) (do (v_of s1) last1) (do (v_of s2') last2))))
          (ensures (eq (do (concrete_merge (v_of lca) (do (v_of s1) last1) (v_of s2)) last2)
                       (concrete_merge (v_of lca) (do (v_of s1) last1) (do (v_of s2) last2)))) = ()
-  
+
 let rec lem_l2a_l1r_eq''_s10 (lca s1 s2:st) (last1 last2:op_t)
   : Lemma (requires ops_of s1 = ops_of lca /\
                     is_prefix (ops_of lca) (ops_of s2) /\
@@ -341,8 +228,7 @@ let rec lem_l2a_l1r_eq''_s10 (lca s1 s2:st) (last1 last2:op_t)
   if ops_of s2 = ops_of lca then
      lem_l2a_l1r_eq''_base lca s1 s2 last1 last2
   else 
-    (assert (length (ops_of s2) > length (ops_of lca)); 
-     let s2' = inverse_st s2 in
+    (let s2' = inverse_st s2 in
      lem_l2a_l1r_eq''_s10 lca s1 s2' last1 last2;
      lem_l2a_l1r_eq''_s10_s2_gt0 lca s1 s2 last1 last2)
 
@@ -381,8 +267,6 @@ let lem_l2a_l1r_eq (lca s1 s2:st)
                     (let _, last1 = un_snoc (ops_of s1) in
                      let _, last2 = un_snoc (ops_of s2) in
                      Add? (snd last2) /\ Rem? (snd last1) /\ get_ele last1 = get_ele last2 /\
-                     //fst last1 <> fst last2 /\
-                     //last (resolve_conflict last1 last2) = last2 /\
                      is_prefix (ops_of lca) (ops_of (inverse_st s2)) /\
                      is_prefix (ops_of lca) (ops_of (inverse_st s1))))
           (ensures (let _, last2 = un_snoc (ops_of s2) in
@@ -400,7 +284,6 @@ let lem_l2a_l1r_eq (lca s1 s2:st)
 
 ///////////////////////////////////////////
 
-#push-options "--z3rlimit 50"
 let lem_l1a_l2r_eq''_base_ind (lca s1 s2:st) (last1 last2:op_t)
   : Lemma (requires length (ops_of lca) > 0 /\
                     ops_of s1 = ops_of lca /\ ops_of s2 = ops_of lca /\
@@ -417,14 +300,11 @@ let lem_l1a_l2r_eq''_base_ind (lca s1 s2:st) (last1 last2:op_t)
           (ensures eq (do (concrete_merge (v_of lca) (v_of s1) (do (v_of s2) last2)) last1)
                       (concrete_merge (v_of lca) (do (v_of s1) last1) (do (v_of s2) last2))) = 
   let pre, lastl = un_snoc (ops_of lca) in
-  lemma_mem_append pre (create 1 lastl);
-  assert (mem lastl (ops_of lca)); 
   lem_mem_ele_mem_id_single lastl (ops_of lca);
   assert (mem_id (fst lastl) (ops_of lca)); 
   assert (fst lastl <> fst last1);
   assert (fst lastl <> fst last2);
   ()
-#pop-options
 
 let rec lem_l1a_l2r_eq''_base (lca s1 s2:st) (last1 last2:op_t)
   : Lemma (requires ops_of s1 = ops_of lca /\ ops_of s2 = ops_of lca /\
@@ -466,8 +346,7 @@ let rec lem_l1a_l2r_eq''_s20 (lca s1 s2:st) (last1 last2:op_t)
   if ops_of s1 = ops_of lca then
      lem_l1a_l2r_eq''_base lca s1 s2 last1 last2
   else 
-    (assert (length (ops_of s1) > length (ops_of lca)); 
-     let s1' = inverse_st s1 in
+    (let s1' = inverse_st s1 in
      lem_l1a_l2r_eq''_s20 lca s1' s2 last1 last2;
      lem_l1a_l2r_eq''_s20_s1_gt0 lca s1 s2 last1 last2)
 
@@ -496,8 +375,7 @@ let rec lem_l1a_l2r_eq'' (lca s1 s2:st) (last1 last2:op_t)
     lem_l1a_l2r_eq''_base lca s1 s2 last1 last2
   else if ops_of s2 = ops_of lca then
     lem_l1a_l2r_eq''_s20 lca s1 s2 last1 last2
-  else (assert (length (ops_of s2) > length (ops_of lca));
-        let s2' = inverse_st s2 in
+  else (let s2' = inverse_st s2 in
         lem_l1a_l2r_eq'' lca s1 s2' last1 last2;
         lem_l1a_l2r_eq''_s2_gt0 lca s1 s2 last1 last2)
         
@@ -506,8 +384,6 @@ let lem_l1a_l2r_eq (lca s1 s2:st)
                     (let _, last1 = un_snoc (ops_of s1) in
                      let _, last2 = un_snoc (ops_of s2) in
                      Add? (snd last1) /\ Rem? (snd last2) /\ get_ele last1 = get_ele last2 /\
-                     //fst last1 <> fst last2 /\
-                     //last (resolve_conflict last1 last2) = last2 /\
                      is_prefix (ops_of lca) (ops_of (inverse_st s2)) /\
                      is_prefix (ops_of lca) (ops_of (inverse_st s1))))
           (ensures (let _, last1 = un_snoc (ops_of s1) in
@@ -628,8 +504,7 @@ let rec lem_l2r_s10 (lca s1 s2:st) (last2:op_t)
    if ops_of s2 = ops_of lca
      then lem_l2r_s10_base lca s1 s2 last2
    else 
-     (assert (length (ops_of s2) > length (ops_of lca));
-      let s2' = inverse_st s2 in
+     (let s2' = inverse_st s2 in
       common_pre1_pre2 lca s1 s2;
       lem_common_pre1_s2' lca s1 s2 last2;
       lem_l2r_s10 lca s1 s2' last2;
@@ -749,34 +624,9 @@ let lem_l2r_l1r_eq (lca s1 s2:st)
                     let s2' = inverse_st s2 in
                     eq (do (concrete_merge (v_of lca) (v_of s1) (v_of s2')) last2)
                        (concrete_merge (v_of lca) (v_of s1) (v_of s2)))) =
-  let pre2, last2 = un_snoc (ops_of s2) in
-  let pre1, last1 = un_snoc (ops_of s1) in
-  let s2' = inverse_st s2 in
-  let s1' = inverse_st s1 in
+  let s1' = inverse_st s1 in //check why this line is needed
   lem_last (ops_of s2);
-  do_prop (v_of s2') last2;
-  assert (forall e. (L.mem e (v_of s2') /\ snd e <> get_ele last2) <==> L.mem e (v_of s2));
-  assert (forall e. L.mem e (diff_s (v_of s2) (v_of lca)) <==>
-               L.mem e (diff_s (v_of s2') (v_of lca)) /\ snd e <> get_ele last2);
-  lem_last (ops_of s1);
-  do_prop (v_of s1') last1;
-  assert (not (mem_ele (get_ele last1) (v_of s1)));
-  assert (not (mem_ele (get_ele last2) (diff_s (v_of s1) (v_of lca)))); 
-  assert (forall e. ((L.mem e (v_of lca) /\ L.mem e (v_of s1) /\ L.mem e (v_of s2')) /\ snd e <> get_ele last2) <==>
-               (L.mem e (v_of lca) /\ L.mem e (v_of s1) /\ L.mem e (v_of s2)));   
-  assert (forall e. L.mem e (concrete_merge (v_of lca) (v_of s1) (v_of s2)) <==>
-               (L.mem e (concrete_merge (v_of lca) (v_of s1) (v_of s2')) /\ snd e <> get_ele last2));
-
-  do_prop (concrete_merge (v_of lca) (v_of s1) (v_of s2')) last2;
-  assert (forall e. (L.mem e (concrete_merge (v_of lca) (v_of s1) (v_of s2')) /\ snd e <> get_ele last2) <==>
-                L.mem e (do (concrete_merge (v_of lca) (v_of s1) (v_of s2')) last2)); 
-
-  trans_op_ele (concrete_merge (v_of lca) (v_of s1) (v_of s2)) 
-               (concrete_merge (v_of lca) (v_of s1) (v_of s2'))
-               (do (concrete_merge (v_of lca) (v_of s1) (v_of s2')) last2)
-               (get_ele last2);
-  assert (eq (do (concrete_merge (v_of lca) (v_of s1) (v_of s2')) last2)
-             (concrete_merge (v_of lca) (v_of s1) (v_of s2))); ()
+  lem_last (ops_of s1)
 
 let lem_l2r_neq_p1 (lca s1 s2:st)
  : Lemma (requires common_pre_s2_gt0 lca s1 s2 /\ 
@@ -833,19 +683,6 @@ let lem_l2r_neq_p2 (lca s1 s2:st)
  assert ((diff (ops_of s1') (ops_of lca)) = pre1d);
  lem_l2r_neq_p2' (diff (ops_of s1) (ops_of lca)) last2
 
-let lem_not_ele_diff1 (lca s1 s2 m:concrete_st) (ele:nat)
-  : Lemma (requires not (mem_ele ele m) /\
-                    eq m (concrete_merge lca s1 s2) /\
-                    not (mem_ele ele (diff_s s2 lca)) /\
-                    (forall e. L.mem e lca /\ L.mem e s1 /\ L.mem e s2 ==> snd e <> ele))
-          (ensures not (mem_ele ele (diff_s s1 lca))) = ()
-
-let lem_not_ele_diff (s1' s1 lca:concrete_st) (op:op_t) (ele:nat)
-  : Lemma (requires s1 == do s1' op /\ get_ele op <> ele /\
-                    not (mem_ele ele (diff_s s1' lca)))
-          (ensures not (mem_ele ele (diff_s s1 lca))) = ()
-
-#push-options "--z3rlimit 50"
 let lem_l2r_ind (lca s1 s2:st)
   : Lemma (requires (Seq.length (ops_of s1) > Seq.length (ops_of lca) /\
                     (let s1' = inverse_st s1 in
@@ -863,24 +700,10 @@ let lem_l2r_ind (lca s1 s2:st)
                     let s2' = inverse_st s2 in
                     eq (do (concrete_merge (v_of lca) (v_of s1) (v_of s2')) last2)
                        (concrete_merge (v_of lca) (v_of s1) (v_of s2)))) =
-  let _, last2 = un_snoc (ops_of s2) in 
-  let s2' = inverse_st s2 in 
-  lem_last (ops_of s2); 
-  do_prop (v_of s2') last2; 
-  assert (not (mem_ele (get_ele last2) (v_of s2)));
-  assert (not (mem_ele (get_ele last2) (diff_s (v_of s2) (v_of lca))));
-  let _, last1 = un_snoc (ops_of s1) in
-  let s1' = inverse_st s1 in
-  lem_last (ops_of s1);
-  do_prop (concrete_merge (v_of lca) (v_of s1') (v_of s2')) last2;
-  assert (not (mem_ele (get_ele last2) (do (concrete_merge (v_of lca) (v_of s1') (v_of s2')) last2))); 
-  assert (forall e. L.mem e (v_of lca) /\ L.mem e (v_of s1') /\ L.mem e (v_of s2) ==> snd e <> get_ele last2); 
-  lem_not_ele_diff1 (v_of lca) (v_of s1') (v_of s2) (do (concrete_merge (v_of lca) (v_of s1') (v_of s2')) last2) (get_ele last2);
-  assert (not (mem_ele (get_ele last2) (diff_s (v_of s1') (v_of lca)))); 
-  lem_not_ele_diff (v_of s1') (v_of s1) (v_of lca) last1 (get_ele last2);
-  assert (not (mem_ele (get_ele last2) (diff_s (v_of s1) (v_of lca))));
-  ()
-#pop-options
+  let s2' = inverse_st s2 in  //check why this line is needed
+  lem_last (ops_of s2);
+  let s1' = inverse_st s1 in //check why this line is needed
+  lem_last (ops_of s1)
 
 let rec lem_l2r' (lca s1 s2:st)
  : Lemma (requires common_pre_s2_gt0 lca s1 s2 /\ 
@@ -900,8 +723,7 @@ let rec lem_l2r' (lca s1 s2:st)
       lem_l2r_s10p lca s1 s2;
       lem_l2r_s10 lca s1 s2' last2) 
    else 
-     (assert ((length (ops_of s1) > length (ops_of lca)));
-      let _, last1 = un_snoc (ops_of s1) in
+     (let _, last1 = un_snoc (ops_of s1) in
       not_add_eq lca s1 s2;
       assert (~ (Add? (snd last1) /\ get_ele last1 = get_ele last2));
       let s1' = inverse_st s1 in
@@ -1084,8 +906,7 @@ let rec lem_l2a''_s20 (lca s1 s2:st) (last2:op_t)
   if ops_of s1 = ops_of lca then 
     lem_l2a''_s20_base lca s1 s2 last2
   else 
-    (assert (length (ops_of s1) > length (ops_of lca));
-     let s1' = inverse_st s1 in
+    (let s1' = inverse_st s1 in
      pre2_pre1_s1 lca s1 s2;
      pre1_pre2_s1 lca s1 s2;
      assert (common_pre_nc lca s1' s2);
@@ -1110,8 +931,7 @@ let rec lem_l2a'' (lca s1 s2:st) (last2:op_t)
   if ops_of s2 = ops_of lca then
     lem_l2a''_s20 lca s1 s2 last2
   else 
-    (assert (length (ops_of s2) > length (ops_of lca));
-     pre2_pre1_s2 lca s1 s2;
+    (pre2_pre1_s2 lca s1 s2;
      assert (common_pre_s2_gt0 lca s1 s2);
      let s2' = inverse_st s2 in
      pre1_pre2_s2 lca s1 s2;
@@ -1162,10 +982,6 @@ let lem_exists (lastop:op_t) (l:log)
                     (forall r. mem r suf /\ get_ele r = get_ele lastop ==> Add? (snd r))))))
   = ()
 
-(*let lem_exists_last_rem (lastop:log_entry) (l:log)
-  : Lemma (requires exists_triple lastop l)
-          (ensures Rem? (snd lastop)) = ()*)
-
 let linearizable_gt0_s1'_op (lca s1 s2:st)
   : Lemma (requires common_pre lca s1 s2 /\ 
                     (let _, last1 = un_snoc (ops_of s1) in
@@ -1182,7 +998,6 @@ let linearizable_gt0_s1'_op (lca s1 s2:st)
   let _, last1 = un_snoc (ops_of s1) in
   let pre2, op2, suf2 = find_triple last1 (diff (ops_of s2) (ops_of lca)) in
   let s2' = inverse_st_op s2 op2 in
-  //lem_exists_last_rem last1 (diff (ops_of s2) (ops_of lca));
   lem_exists last1 (diff (ops_of s2) (ops_of lca));
   lem_inverse (ops_of lca) (ops_of s1);
   lem_diff (ops_of s1) (ops_of lca);
@@ -1209,7 +1024,6 @@ let linearizable_gt0_s2'_op (lca s1 s2:st)
   let _, last2 = un_snoc (ops_of s2) in
   let pre1, op1, suf1 = find_triple last2 (diff (ops_of s1) (ops_of lca)) in
   let s1' = inverse_st_op s1 op1 in
-  //lem_exists_last_rem last2 (diff (ops_of s1) (ops_of lca));
   lem_exists last2 (diff (ops_of s1) (ops_of lca));
   lem_inverse (ops_of lca) (ops_of s2);
   lem_diff (ops_of s2) (ops_of lca);
@@ -1306,30 +1120,20 @@ let linearizable_gt0_s2' (lca s1 s2:st)
 //// Sequential implementation //////
 
 // the concrete state 
-let concrete_st_s = list nat
+let concrete_st_s = S.set nat
 
 // init state 
-let init_st_s = []
-
-val filter_seq : f:(nat -> bool)
-               -> l:concrete_st_s
-               -> Tot (l1:concrete_st_s {(forall e. L.mem e l1 <==> L.mem e l /\ f e)})
-let rec filter_seq f l = 
-  match l with
-  |[] -> []
-  |hd::tl -> if f hd then hd::(filter_seq f tl) else filter_seq f tl
-  
+let init_st_s = S.empty
+ 
 // apply an operation to a state 
-let do_s (st_s:concrete_st_s) (o:op_t) 
-  : (r:concrete_st_s{(Add? (snd o) ==> (forall e. L.mem e r <==> L.mem e st_s \/ e = get_ele o)) /\
-                     (Rem? (snd o) ==> (forall e. L.mem e r <==> L.mem e st_s /\ e <> get_ele o))}) =
+let do_s (st_s:concrete_st_s) (o:op_t) : concrete_st_s =
   match snd o with
-  |(Add e) -> e::st_s
-  |(Rem e) -> filter_seq (fun ele -> ele <> e) st_s
+  |(Add e) -> S.union (S.singleton e) st_s
+  |(Rem e) -> remove_if st_s (fun ele -> ele = e) 
 
 //equivalence relation between the concrete states of sequential type and MRDT
 let eq_sm (st_s:concrete_st_s) (st:concrete_st) =
-  (forall e. L.mem e st_s <==> mem_ele e st)
+  (forall e. S.mem e st_s <==> mem_ele e st)
 
 //initial states are equivalent
 let initial_eq (_:unit)
@@ -1342,45 +1146,3 @@ let do_eq (st_s:concrete_st_s) (st:concrete_st) (op:op_t)
 
 ////////////////////////////////////////////////////////////////
 
-(*let rem_add_lastop_neq_ele (lca s1 s2:st)
-  : Lemma (requires Seq.length (ops_of s1) > Seq.length (ops_of lca) /\
-                    common_pre_s2_gt0 lca s1 s2 /\
-                    (let _, last2 = un_snoc (ops_of s2) in
-                    let _, last1 = un_snoc (ops_of s1) in
-                    Add? (snd last2) /\
-                    not (exists_triple last2 (diff (ops_of s1) (ops_of lca))) /\
-                    not (exists_triple last1 (diff (ops_of s2) (ops_of lca)))))
-          (ensures (let _, last2 = un_snoc (ops_of s2) in
-                    let _, last1 = un_snoc (ops_of s1) in
-                    ~ (Rem? (snd last1) /\ get_ele last1 = get_ele last2))) =
-  let _, last2 = un_snoc (ops_of s2) in
-  let _, last1 = un_snoc (ops_of s1) in
-  lastop_neq (ops_of lca) (ops_of s1) (ops_of s2);
-  resolve_conflict_prop last1 last2;
-  assert (fst last1 <> fst last2);
-
-  let s2' = inverse_st s2 in
-  lemma_mem_snoc (ops_of s2') last2;
-  assert (mem last2 (ops_of s2));
-  lem_last (ops_of s2);
-  assert (last (ops_of s2) = last2);
-  lem_diff (ops_of s2) (ops_of lca);
-  assert (last (diff (ops_of s2) (ops_of lca)) = last2);
-  assert (mem last2 (diff (ops_of s2) (ops_of lca)));
-  let pre, suf = pre_suf (diff (ops_of s2) (ops_of lca)) last2 in
-  lem_lastop_suf_0 (diff (ops_of s2) (ops_of lca)) pre suf last2;
-  assert (length suf = 0);
-  lemma_empty suf; 
-  comm_empty_log last2 suf; 
-  
-  assert (Rem? (snd last1) /\ get_ele last1 = get_ele last2 ==> commutative_seq last2 suf); 
-  assert (Rem? (snd last1) /\ get_ele last1 = get_ele last2 ==> not (commutative last1 last2));
-  assert (Rem? (snd last1) /\ get_ele last1 = get_ele last2 ==> last (resolve_conflict last1 last2) = last2);
-  assert (Rem? (snd last1) /\ get_ele last1 = get_ele last2 ==> 
-          (not (commutative last1 last2) /\
-          last (resolve_conflict last1 last2) = last2 /\
-          commutative_seq last2 suf));
-  assert (Rem? (snd last1) /\ get_ele last1 = get_ele last2 ==> 
-           exists_triple last1 (diff (ops_of s2) (ops_of lca)));
-  ()*)
-         
